Proof of decoder invariants complete + func model changes
Needs to be cleaned up but no more admits

Made a few changes to functional models:
1. Changed check for existence to \in rather than Znth, will
   need to prove equivalent later.
2. Add packet to block even if block complete (needed to ensure
   that count is correct).
3. Was deleting blocks in [update_dec_state] inductive case, fixed
   this bug.

Should put lemma about distance between packets into new lemma, use
to prove equiv with no timeouts

proofs/FEC/DecoderGeneric.v
@@ -215,9 +215,13 @@ Definition add_fec_packet_to_block (p: fpacket) (b: block) : block :=
       <| parity_packets := sublist (blk_k b) (blk_k b + blk_h b) new_packets |>.
 
 Definition add_packet_to_block_black (p: fpacket) (b: block) : block * list packet :=
-  if black_complete b then (b, if (fd_isParity p) then nil else [p_packet p]) else 
-    (*NOTE: theirs does not release data packet here*)
-    let new_block := add_fec_packet_to_block p b in 
+  (*NOTE: we still must add the packet even if the block is complete
+    to keep the time correctly updated. But we don't need to output anything*)
+  let new_block := add_fec_packet_to_block p b in
+  if black_complete b then (new_block, if (fd_isParity p) then nil else [p_packet p]) else 
+    (*NOTE: theirs does not release data packet here - we can do either, the
+      block has been recovered so this would just be a duplicate. But
+      not returning anything does violate their stated spec*)
     let packets := (if (fd_isParity p) then nil else [p_packet p]) ++
       (if recoverable new_block then (decode_block new_block) else nil) in
     let marked_block := if recoverable new_block then new_block <| black_complete := true |> else new_block in
@@ -283,7 +287,9 @@ Fixpoint update_dec_state_gen (blocks: list block) (curr: fpacket)
     else if (currSeq < (blk_id bl))%N then 
       let t := create_block_with_packet_black curr time in 
         (t.1 :: blocks, t.2)
-    else update_dec_state_gen tl curr time
+    else 
+      let t := update_dec_state_gen tl curr time
+      in (bl :: t.1, t.2)
   end.
 
 Definition decoder_one_step_gen (blocks: list block) curr time :
@@ -363,6 +369,31 @@ Qed.
 
 (*sortedness*)
 
+(*TODO: we prove a stronger version later: combine?*)
+Lemma in_update_dec_state_gen_id: forall b blks (p: fpacket) time,
+  b \in (update_dec_state_gen blks p time).1 ->
+  fd_blockId p = blk_id b \/
+  exists b', (b' \in blks) && (blk_id b' == blk_id b).
+Proof.
+  move=> b blks p time. elim: blks => [//= | bhd btl /= IH].
+  - rewrite in_cons orbF => /eqP ->.
+    left. by case: (Z.eq_dec (fd_k p) 1).
+  - case: (fd_blockId p == blk_id bhd) /eqP => Hid.
+    + rewrite in_cons => /orP[/eqP Hb | Hinb].
+      * left. subst. by rewrite Hid add_packet_to_block_black_id.
+      * right. exists b. by rewrite in_cons Hinb orbT eq_refl.
+    + case Hlt: (fd_blockId p < blk_id bhd)%N=>/=.
+      * rewrite !in_cons => /orP[ /eqP -> |/orP[/eqP->|Hinb]].
+        -- left. by case: (Z.eq_dec (fd_k p) 1).
+        -- right. exists bhd. by rewrite mem_head eq_refl.
+        -- right. exists b. by rewrite in_cons Hinb orbT eq_refl.
+      * rewrite in_cons => /orP[/eqP -> | Hinb].
+        -- right. exists bhd. by rewrite mem_head eq_refl.
+        -- move: IH => /(_ Hinb) [Hpb | [b' /andP[Hinb' Hb']]].
+          ++ by left.
+          ++ right. exists b'. by rewrite in_cons Hinb' orbT.
+Qed.
+
 Definition blk_order: rel block :=
   (fun x y => ((blk_id x) < (blk_id y))%N).
 (*Should make block IDs nats, do everything in terms of nats*)
@@ -393,10 +424,20 @@ Proof.
     move: Hpath.
     case: btl => //= bhd' btl /andP[Hlt Hpath].
     rewrite Hpath andbT. by rewrite add_packet_to_block_black_id.
-  - case Hlt: ((fd_blockId curr) < (blk_id bhd))%N; last by apply IH.
-    by case Hk1: (proj_sumbool (Z.eq_dec (fd_k curr) 1))=>/=; rewrite Hlt/=;
-    apply (@path_filter_in _ xpredT).
-Qed.
+  - case Hlt: ((fd_blockId curr) < (blk_id bhd))%N=>/=.
+    + by case Hk1: (proj_sumbool (Z.eq_dec (fd_k curr) 1))=>/=; rewrite Hlt/=;
+      apply (@path_filter_in _ xpredT).
+    + move: IH => /(_ Htl). move: Hpath.
+      rewrite !path_sortedE; try by move=> b1 b2 b3; apply ltn_trans.
+      move=>/andP[/allP Hall _] Hsort.  
+      rewrite Hsort andbT.
+      apply /allP => b1 Hinb1.
+      apply in_update_dec_state_gen_id in Hinb1.
+      case: Hinb1 => [Hcurr | [b' /andP[Hinb' /eqP Hb']]].
+      * by rewrite -Hcurr ltnNge leq_eqVlt Hlt (introF eqP Heq).
+      * rewrite -Hb'. apply Hall.
+        by move: Hinb'; rewrite mem_filter => /andP[_ ].
+Qed.  
 
 (*From this, we get uniqueness for free*)
 
@@ -797,57 +838,7 @@ Proof.
       by rewrite in_cons Hinpl orbT. by rewrite mem_head.
       by rewrite Hidp. } rewrite Hk Hh.
     have Hlenpkts: Zlength pkts = fd_k h + fd_h h. rewrite -Hk -Hh. apply (Hlen _ _ _ Hint Hinp).
-    rewrite /subblock/=. split.
-      move: Hsub. by rewrite /subblock Hb2 //= => [[H _]].
-    move: Hpos => /( _ h (mem_head _ _)) => Hbounds.
-    rewrite !cat_app -sublist_split; try lia.
-    rewrite !(sublist_same 0 (fd_k h + fd_h h)) //.
-    move: Hsub. rewrite /subblock => [[Hid [Hdat [Hpars [Hks Hhs]]]]].
-    have Hbounds': 0 <= Z.of_nat (fd_blockIndex h) < fd_k h + fd_h h.
-      split; try lia; apply Hwf. by rewrite in_cons eq_refl.
-    (*we need to know the relationship between data_packets, parity_packets, etc*)
-    subst; simpl in *.
-    (*Do this so we don't need to prove same things twice:*)
-    have Hsubupd: forall lo hi l, 0 <= Z.of_nat (fd_blockIndex h) < Zlength pkts -> 0 <= lo <= hi ->
-        hi <= Zlength pkts ->
-        subseq_option l (sublist lo hi pkts) ->
-        subseq_option l (sublist lo hi (upd_Znth (Z.of_nat (fd_blockIndex h)) pkts (Some h))). {
-      move => lo hi l1 Hhhi Hlohi Hhilen. 
-      rewrite /subseq_option !Zlength_sublist; try lia; [|list_solve] => [[Hlens Hith]]. split. lia.
-      move => j Hj.
-      have [Hin | [Hout1 | Hout2]]: lo <= Z.of_nat (fd_blockIndex h) < hi \/
-        0 <= Z.of_nat (fd_blockIndex h) < lo \/ hi <= Z.of_nat (fd_blockIndex h) < Zlength pkts by lia.
-      * rewrite sublist_upd_Znth_lr; try lia.
-        rewrite (upd_Znth_lookup' (hi - lo)); try lia; [|list_solve].
-        case : (Z.eq_dec j (Z.of_nat (fd_blockIndex h) - lo)) => Hjh.
-        -- (*the key part: Znth j (data_packets b1) MUST be None or Some h, since if it is anything else,
-              pkts will not a well-formeed packet list -conradicts uniquenss*)
-          case Hjth: (Znth j l1) => [p' |//]; last first. by right.
-          left. f_equal.
-          move : Hith => /(_ j Hj). rewrite Znth_sublist; try lia.
-          have->: j + lo = Z.of_nat (fd_blockIndex h) by lia.
-          rewrite Hjth => [[Hjth' | //]]. apply esym in Hjth'.
-          have Hinj: (Some p') \in pkts. rewrite -Hjth'. apply /inP. 
-            apply Znth_In. simpl in *; lia.
-          have [Hidp' Hinlp']: fd_blockId p' = fd_blockId p /\ p' \in l by 
-            apply (@get_block_lists_prop_packets l (get_block_lists l) (fd_blockId p) pkts).
-          apply Hwf.
-          ++ by rewrite in_cons Hinlp' orbT.
-          ++ by rewrite mem_head.
-          ++ by rewrite Hidp'.
-          ++ move: Hjth'. rewrite (Heq _ _ Hint). rewrite mkseqZ_Znth; try lia.
-              case_pickSeq l => [[Hxp]|//]. rewrite -Hxp. solve_sumbool.
-              by apply Nat2Z.inj in e. 
-        -- by apply Hith.
-      * rewrite sublist_upd_Znth_r; try lia. by apply Hith.
-      * rewrite sublist_upd_Znth_l; try lia. by apply Hith.
-    } 
-    split_all.
-    + apply Hsubupd; try lia. by rewrite -Hk.
-    + apply Hsubupd; try lia. by rewrite -Hh -Hk.
-    + lia.
-    + lia.
-    + simpl in *; lia.
+    apply subblock_add. by rewrite -Hk -Hh-Hb2.
 Qed.
 
 Opaque create_block_with_packet_black.
@@ -876,15 +867,37 @@ Proof.
         move: Hsubs => /(_ b Hin') [b1 [Hinb1 Hsub1]].
         have [b2 [Hinb2 Hsub2]]:=(get_blocks_sublist Hwf Hht Hinb1).
         exists b2. split => //. by apply (subblock_trans Hsub1).
-    + case Hlt: (fd_blockId curr < blk_id h)%N; last by
-        apply IH =>// b' Hin; apply Hsubs; rewrite in_cons Hin orbT.
-      rewrite in_cons => /orP[/eqP Hb | Hin].
-      * rewrite Hb. apply create_block_subblock => //. 
-        by rewrite mem_head.
-      * move: Hsubs => /(_ b Hin) [b1 [Hinb1 Hsub1]].
-        have [b2 [Hinb2 Hsub2]]:=(get_blocks_sublist Hwf Hht Hinb1).
-        exists b2. split => //. by apply (subblock_trans Hsub1).
+    + case Hlt: (fd_blockId curr < blk_id h)%N.
+      * rewrite in_cons => /orP[/eqP Hb | Hin].
+        -- rewrite Hb. apply create_block_subblock => //. 
+          by rewrite mem_head.
+        -- move: Hsubs => /(_ b Hin) [b1 [Hinb1 Hsub1]].
+          have [b2 [Hinb2 Hsub2]]:=(get_blocks_sublist Hwf Hht Hinb1).
+          exists b2. split => //. by apply (subblock_trans Hsub1).
+      * rewrite in_cons => /orP[/eqP Hbh | Hin].
+        -- subst.
+          move: Hsubs => /(_ h (mem_head _ _)) [b1 [Hinb1 Hsub1]].
+          have [b2 [Hinb2 Hsub2]]:=(get_blocks_sublist Hwf Hht Hinb1).
+          exists b2. split=>//. by apply (subblock_trans Hsub1).
+        -- by apply (IH time) =>// b' Hin'; apply Hsubs; 
+          rewrite in_cons Hin' orbT.
 Qed.
+
+(*A very easy corollary, but we need it in the decoder timeout
+  invariant*)
+Lemma decoder_one_step_gen_subblocks: forall l blks curr time,
+  wf_packet_stream (curr :: l) ->
+  (forall b, b \in blks -> exists b', b' \in (get_blocks l) /\ subblock b b') ->
+  forall b, b \in (decoder_one_step_gen blks curr time).1.1 ->
+    exists b', b' \in (get_blocks (curr :: l)) /\ subblock b b'.
+Proof.
+  move=> l blks curr time Hwf Hsubs b.
+  rewrite /decoder_one_step_gen.
+  apply (update_dec_state_gen_subblocks Hwf).
+  move => b'. rewrite mem_filter => /andP[_ Hinb'].
+  by apply Hsubs.
+Qed.
+
 
   (*NOTE: one reason why this is better is because we no longer have
     external state in the decoder that we have to reason about*)
@@ -926,9 +939,9 @@ Proof.
    z.2 ++ [:: x0])) ([::], [::], 0, [::]) t).
   (*We don't care what blks is. It is long and ugly, so we generalize*)
   move: blks => blks IH Hinb.
-  eapply (update_dec_state_gen_subblocks Hwf). 2: apply Hinb.
-  move => b'. rewrite mem_filter => /andP[_ Hinb'].
-  apply IH =>//. exact (wf_packet_stream_tl Hwf).
+  eapply decoder_one_step_gen_subblocks. apply Hwf.
+  2: apply Hinb. move=> b'. apply IH.
+  exact (wf_packet_stream_tl Hwf).
 Qed.
 
 (*The other general result we need: we need to relate the output
@@ -1059,7 +1072,10 @@ Proof.
           move: Hin; rewrite !in_cons orbF => /eqP->.
           by rewrite eq_refl.
         -- by right.
-      * by apply IH.
+      * apply IH in Hin. 
+        case: Hin => [[b' [Hinb' [Hrec Hdec]]]| [Hcurr Hpar]].
+        -- left. exists b'. by rewrite in_cons Hinb' orbT.
+        -- by right.
 Qed. 
 
 Theorem in_decode_func_in_block: forall received (curr: fpacket) (p: packet),
@@ -1163,14 +1179,283 @@ Proof.
           ++ left. by rewrite Hb.
           ++ rewrite mem_filter => /andP[Hfb Hinb].
             left. by rewrite Hinb orbT.
-        -- move=> Hinb. apply IH in Hinb=>//.
-          case: Hinb => [Htl | [[Hb Hall]| [b' [Hinb' Hb']]]].
-          ++ left. by rewrite in_cons Htl orbT.
-          ++ right. left. split=>//. move=>b'. 
-            rewrite in_cons => /orP[/eqP Hb' | Hinb']; subst.
-            right. by case: (Z.eq_dec (fd_k p) 1) =>/= _; auto.
-            by apply Hall.
-          ++ right. right. exists b'. by rewrite in_cons Hinb' orbT.
+        -- rewrite in_cons => /orP[/eqP Hbhd | Hinb]; first by
+            left; subst; rewrite mem_head.
+          apply IH in Hinb=>//.
+            case: Hinb => [Htl | [[Hb Hall]| [b' [Hinb' Hb']]]].
+            ++ left. by rewrite in_cons Htl orbT.
+            ++ right. left. split=>//. move=>b'. 
+              rewrite in_cons => /orP[/eqP Hb' | Hinb']; subst.
+              right. by case: (Z.eq_dec (fd_k p) 1) =>/= _; auto.
+              by apply Hall.
+            ++ right. right. exists b'. by rewrite in_cons Hinb' orbT.
 Qed.
+
+Lemma packet_in_create: forall s (p: fpacket) time,
+  wf_packet_stream s ->
+  p \in s ->
+  packet_in_block p (create_block_with_packet_black p time).1.
+Proof.
+  move=> s p time Hwf Hinp.
+  case: Hwf => [_ [_ [/(_ _ Hinp) Hidx /(_ _ Hinp) Hnonneg]]].
+  rewrite /create_block_with_packet_black packet_in_block_eq/=.
+  case: (Z.eq_dec (fd_k p) 1)=>//= _;
+  (*Both cases are the exact same*)
+  apply /orP; rewrite !in_mem_In; apply in_app_or;
+  rewrite -sublist_split; try lia; (try by 
+    rewrite Zlength_upd_Znth zseq_Zlength; lia);
+  rewrite sublist_same; try lia; (try by
+    rewrite Zlength_upd_Znth zseq_Zlength; lia);
+  apply upd_Znth_In; rewrite zseq_Zlength; lia.
+Qed.
+
+Lemma packet_in_add: forall s (p: fpacket) b,
+  wf_packet_stream s ->
+  p \in s ->
+  fd_k p = blk_k b ->
+  fd_h p = blk_h b ->
+  Zlength (data_packets b) = blk_k b ->
+  Zlength (parity_packets b) = blk_h b ->
+  packet_in_block p (add_fec_packet_to_block p b).
+Proof.
+  move=> s p b Hwf Hinp Hk Hh Hdat Hlen.
+  case: Hwf => [_ [_ [/(_ _ Hinp) Hidx /(_ _ Hinp) Hnonneg]]]. 
+  rewrite /add_fec_packet_to_block packet_in_block_eq/=.
+  apply /orP. rewrite !in_mem_In !cat_app; apply in_app_or.
+  rewrite -sublist_split; try lia; last by
+    (simpl in *; list_solve).
+  rewrite sublist_same; try lia; last by (simpl in *; list_solve).
+  apply upd_Znth_In. simpl in *; list_solve.
+Qed.
+
+Lemma packet_in_add_black: forall s (p: fpacket) b,
+  wf_packet_stream s ->
+  p \in s ->
+  fd_k p = blk_k b ->
+  fd_h p = blk_h b ->
+  Zlength (data_packets b) = blk_k b ->
+  Zlength (parity_packets b) = blk_h b ->
+  packet_in_block p (add_packet_to_block_black p b).1.
+Proof.
+  move=> s p b Hwf Hin Hk Hh Hdat Hpar. 
+  rewrite /add_packet_to_block_black.
+  case: (black_complete b)=>/=. by apply (packet_in_add Hwf).
+  by case: (recoverable (add_fec_packet_to_block p b)); apply (packet_in_add Hwf).
+Qed.
+(*Why do I keep having to do this?*)
+Opaque create_block_with_packet_black.
+
+Ltac pre_impl H :=
+  match goal with
+  | H: ?P -> ?Q |- _ => let name := fresh in 
+    have name: P; [| move: H => /( _ name) H]
+  end.
+
+
+(*There is always a block with the packet that was added*)
+Lemma packet_in_one_step: forall s blocks (p: fpacket) time,
+  wf_packet_stream s ->
+  p \in s ->
+  (forall b' (p': fpacket), p' \in s -> b' \in blocks -> fd_blockId p = blk_id b' ->
+    fd_k p = blk_k b' /\ fd_h p = blk_h b') ->
+  (forall b', b' \in blocks -> Zlength (data_packets b') = blk_k b' /\
+    Zlength (parity_packets b') = blk_h b') ->
+  exists b, (b \in (decoder_one_step_gen blocks p time).1.1) && 
+    (packet_in_block p b).
+Proof.
+  move=> s blks p time Hwf Hinp. 
+  rewrite /decoder_one_step_gen.
+  move: (upd_time time p blks) => upd.
+  move: (not_timeout) => f.
+  elim: blks => [//= Hallkh Halllen | bhd btl /= IH Hallkh Halllen].
+  - exists (create_block_with_packet_black p upd).1.
+    by rewrite mem_head/= (packet_in_create _ Hwf).
+  - (*Lemmas for IH*)
+    pre_impl IH.
+      move=> b' p' Hinp' Hinb' Hideq. apply (Hallkh b' p')=>//.
+      by rewrite in_cons Hinb' orbT.
+    pre_impl IH.
+      move=>b' Hinb'. apply Halllen. by rewrite in_cons Hinb' orbT.
+  case: (f upd bhd)=>//=.
+    + case: (fd_blockId p == blk_id bhd) /eqP => Hids.
+      (*Need the assumptions so that we know that p is in
+        the resulting block*)
+      * exists (add_packet_to_block_black p bhd).1. rewrite mem_head/=.
+        move: Hallkh=>/(_ bhd p Hinp (mem_head _ _) Hids) [Hk Hh].
+        move: Halllen=>/(_ bhd (mem_head _ _)) [Hdat Hpar].
+        by apply (packet_in_add_black Hwf).
+      * case Hlt: (fd_blockId p < blk_id bhd)%N.
+        -- exists (create_block_with_packet_black p upd).1.
+          by rewrite mem_head/= (packet_in_create _ Hwf).
+        -- case: IH => [b' /andP[Hinb' Hinp']].
+          exists b'. by rewrite in_cons Hinb' orbT.
+Qed.
+
+(*TODO: use existsP?*)
+Lemma existsbP: forall {A: eqType} {s: seq A} {P: A -> bool},
+  reflect (exists x, (x \in s) && P x) (existsb P s).
+Proof.
+  move=> A s P. elim: s => [//= | hd tl /= IH].
+  - by apply ReflectF => [[]].
+  - case Hhd: (P hd).
+    + apply ReflectT. exists hd. by rewrite mem_head Hhd.
+    + move: IH. case Htl: (existsb P tl) => IH.
+      * apply ReflectT. apply elimT in IH =>//.
+        case: IH => [x /andP[Hintl Hp]].
+        exists x. by rewrite in_cons Hintl orbT.
+      * apply ReflectF. apply elimF in IH=>//.
+        move => [x]. 
+        rewrite in_cons => /andP[/orP[/eqP Hx | Hintl] Hpx]; subst.
+        by rewrite Hpx in Hhd. apply IH. exists x.
+        by rewrite Hintl Hpx.
+Qed.
+
+(*[update_dec_state_gen] does nothing if all blockIds are*)
+
+(*The included lemma is weaker than it needs to be
+  TODO: replace in VST?*)
+Lemma In_upd_Znth_old': forall {A: Type} {d: Inhabitant A} (i: Z)
+  (x y : A) (l: list A),
+  In x l ->
+  x <> Znth i l ->
+  In x (upd_Znth i l y).
+Proof.
+  intros A d i x y l Hin Hnth.
+  assert (0 <= i <= Zlength l \/ ~(0 <= i <= Zlength l)) 
+    as [Hinb | Houtb] by lia.
+  - apply In_upd_Znth_old; assumption.
+  - rewrite -> upd_Znth_out_of_range by lia. assumption.
+Qed.
+  (*ugh, we need to know the location - see about that, can
+    we prove from [get_blocks]? this may be more annoying also*)
+
+Lemma other_in_add: forall (p p': fpacket) b,
+  fd_blockIndex p <> fd_blockIndex p' ->
+  Zlength (data_packets b) = blk_k b ->
+  Zlength (parity_packets b) = blk_h b ->
+  Znth (Z.of_nat (fd_blockIndex p')) 
+    (data_packets b ++ parity_packets b) = Some p' ->
+  packet_in_block p' (add_fec_packet_to_block p b).
+Proof.
+  move=> p p' b Hpp' Hdat Hpar.
+  rewrite /add_fec_packet_to_block !packet_in_block_eq/==> Hin.
+  apply /orP. rewrite !in_mem_In. 
+  apply in_app_or.
+  (*Can't use [sublist_split] because we don't know bounds*)
+  rewrite -sublist_split; [|list_solve| 
+    rewrite Zlength_upd_Znth cat_app; simpl in *; list_solve].
+  rewrite sublist_same; try lia; last by
+    rewrite Zlength_upd_Znth cat_app; simpl in *; list_solve.
+  apply In_Znth_iff. exists (Z.of_nat (fd_blockIndex p')).
+  rewrite Znth_upd_Znth_diff; last by 
+    move=> C; apply Nat2Z.inj in C; rewrite C in Hpp'.
+  split=>//. rewrite Zlength_upd_Znth.
+  apply Znth_inbounds. by rewrite Hin.
+Qed.
+
+Lemma other_in_add_black: forall (p p': fpacket) b,
+  fd_blockIndex p <> fd_blockIndex p' ->
+  Zlength (data_packets b) = blk_k b ->
+  Zlength (parity_packets b) = blk_h b ->
+  Znth (Z.of_nat (fd_blockIndex p')) 
+    (data_packets b ++ parity_packets b) = Some p' ->
+  packet_in_block p' (add_packet_to_block_black p b).1.
+Proof.
+  move=> p p' b Hpp' Hdat Hpar Hnth.
+  rewrite /add_packet_to_block_black.
+  case: (black_complete b)=>/=; first by apply other_in_add.
+  by case: (recoverable (add_fec_packet_to_block p b));
+    apply other_in_add.
+Qed.
+
+(*Sort of the opposite of [in_decoder_one_step]*)
+(*For every block in blocks, either a version of it containing 
+  the packet p' (different than p) is in
+  the resulting list or it has timed out.*)
+Lemma notin_decoder_one_step: forall blocks (p p': fpacket) time b,
+  (fd_blockId p <> fd_blockId p' \/ fd_blockIndex p <> fd_blockIndex p') ->
+  (forall b', b' \in blocks -> Zlength (data_packets b') = blk_k b' /\
+    Zlength (parity_packets b') = blk_h b') ->
+  (forall b' (p': fpacket), b' \in blocks -> packet_in_block p' b' ->
+    Znth (Z.of_nat (fd_blockIndex p')) 
+      (data_packets b' ++ parity_packets b') = Some p') ->
+  (forall b' (p': fpacket), b' \in blocks -> packet_in_block p' b' ->
+    fd_blockId p' = blk_id b') ->
+  (*sorted blk_order blocks ->*)
+  b \in blocks ->
+  packet_in_block p' b ->
+  ~(exists b, ((b \in (decoder_one_step_gen blocks p time).1.1) && 
+    packet_in_block p' b)) ->
+  not_timeout (upd_time time p blocks) b = false.
+Proof.
+(*  (exists b', (b' \in (decoder_one_step_gen blocks p time).1.1) &&
+    packet_in_block p' b' && not_timeout (upd_time time p blocks) b') \/
+  not_timeout (upd_time time p blocks) b = false.
+Proof.*)
+  move=>blks p p' time b Hpp'/=. move: (upd_time time p blks) => tm.
+  move: not_timeout => f.
+  elim: blks =>[//= | bhd btl /= IH Hlens Hnths Hids (*Hsort*) Hinb Hinp'].
+  (*Instantiate results for IH*)
+  pre_impl IH.
+    by move=> b' Hinb'; apply Hlens; by rewrite in_cons Hinb' orbT.
+  pre_impl IH.
+    by move=> p'' b' Hinb' Hinp''; apply (Hnths p'' b')=>//; 
+    rewrite in_cons Hinb' orbT.
+  pre_impl IH.
+    by move => b' p'' Hinb' Hinp''; apply (Hids b' p'')=>//;
+    rewrite in_cons Hinb' orbT.
+  (*move: Hsort. rewrite path_sortedE; last by move=> b1 b2 b3; apply ltn_trans.
+  move=> /andP[/allP Halllt Hsort].
+  move: IH => /(_ Hsort) IH.*) 
+  move: Hinb; rewrite in_cons => /orP[/eqP Hbhd | Hintl]; last first.
+  - case Htb: (f tm b)=>//=.
+    have Hinf: b \in [seq x <- btl | f tm x] by rewrite mem_filter Htb Hintl.
+    have->: true = false <-> False by []. move=> Hex; apply Hex. rewrite {Hex}.
+    case Hf: (f tm bhd)=>//=.
+    + case Heq: (fd_blockId p == blk_id bhd).
+      * exists b. by rewrite Hinp' andbT in_cons Hinf orbT.
+      * case Hlt: (fd_blockId p < blk_id bhd)%N.
+        -- exists b. by rewrite Hinp' andbT !in_cons Hinf !orbT.
+        -- (*here, we have the IH*)
+          move: IH => /(_ Hintl Hinp') Hex.
+          have [b' /andP[Hinb' Hinp'']]:
+          (exists b : block,
+          (b \in (update_dec_state_gen [seq x <- btl | f tm x] p tm).1) &&
+          packet_in_block p' b). {
+            (*We can eliminate the double negation because this is
+              decidable*)
+            case: (existsb (fun b => packet_in_block p' b)
+              ((update_dec_state_gen [seq x <- btl | f tm x] p tm).1)) 
+              /existsbP=>//.
+            move=> Hnotex. exfalso. rewrite Htb in Hex. 
+            have//: true = false by apply Hex.
+          }
+          exists b'. by rewrite in_cons Hinb' orbT.
+    + (*Again, IH case*)
+      move: IH => /(_ Hintl Hinp') Hex.
+      case: (existsb (fun b => packet_in_block p' b)
+        ((update_dec_state_gen [seq x <- btl | f tm x] p tm).1)) 
+        /existsbP=>//.
+      move=> Hnotex. exfalso. rewrite Htb in Hex. 
+      have//: true = false by apply Hex.
+  - (*Head case*) subst.
+    case Hf: (f tm bhd)=>//.
+    + move=> Hnotex. exfalso. apply Hnotex. rewrite {Hnotex}/=.
+      case: (fd_blockId p == blk_id bhd) /eqP => Heq.
+      * case: Hpp' => [Hnotid | Hnotidx].
+        -- (*must have the same id due to the blocks they are
+          in, so contradiction*)
+          exfalso. apply Hnotid. rewrite Heq. symmetry. 
+          apply (Hids _ _ (mem_head _ _) Hinp').
+        -- (*Otherwise, same idx so we don't overwrite p'*)
+          exists ((add_packet_to_block_black p bhd).1).
+          rewrite mem_head/=.  
+          apply other_in_add_black=>//;
+          try by (apply Hlens; rewrite mem_head).
+          apply (Hnths bhd)=>//. by rewrite mem_head.
+      * case Hlt: (fd_blockId p < blk_id bhd)%N.
+        -- exists bhd. by rewrite !in_cons eq_refl !orbT.
+        -- exists bhd. by rewrite mem_head.
+Qed.  
 
 End GenDecode.
